QsImpl now includes full Tuples2F (warning: I haven't finished building everything all together yet)

Bedrock/Platform/Facade/examples/QsImpl.v
@@ -10,7 +10,7 @@ Require Import Bedrock.Platform.Cito.RepInv Bedrock.Platform.Cito.MakeADT.
 
 Require Import Bedrock.Platform.AutoSep.
 
-Require Import Bedrock.Platform.Facade.examples.ArrayTupleF Bedrock.Platform.Facade.examples.TupleListF Bedrock.Platform.Facade.examples.Tuples0F Bedrock.Platform.Facade.examples.Tuples1F.
+Require Import Bedrock.Platform.Facade.examples.ArrayTupleF Bedrock.Platform.Facade.examples.TupleListF Bedrock.Platform.Facade.examples.Tuples0F Bedrock.Platform.Facade.examples.Tuples1F Bedrock.Platform.Facade.examples.Tuples2F.
 Require Import Bedrock.Platform.Facade.examples.QsRepInv.
 
 Module Import Made := MakeADT.Make(QsADTs.Adt)(Ri).
@@ -56,7 +56,14 @@ Definition m0 := bimport [[ "sys"!"abort" @ [abortS],
                             "Tuples1"!"new" @ [Tuples1F.newS],
                             "Tuples1"!"insert" @ [Tuples1F.insertS],
                             "Tuples1"!"find" @ [Tuples1F.findS],
-                            "Tuples1"!"enumerate" @ [Tuples1F.enumerateS] ]]
+                            "Tuples1"!"enumerate" @ [Tuples1F.enumerateS],
+
+                            "Tuples2"!"new" @ [Tuples2F.newS],
+                            "Tuples2"!"insert" @ [Tuples2F.insertS],
+                            "Tuples2"!"findBoth" @ [Tuples2F.findBothS],
+                            "Tuples2"!"findFirst" @ [Tuples2F.findFirstS],
+                            "Tuples2"!"findSecond" @ [Tuples2F.findSecondS],
+                            "Tuples2"!"enumerate" @ [Tuples2F.enumerateS] ]]
   fmodule "ADT" {{
     ffunction "Tuple_new" reserving 7 [Tuple_new] := "ArrayTuple"!"new"
     with ffunction "Tuple_delete" reserving 6 [Tuple_delete] := "ArrayTuple"!"delete"
@@ -81,6 +88,13 @@ Definition m0 := bimport [[ "sys"!"abort" @ [abortS],
     with ffunction "Tuples1_insert" reserving 21 [Tuples1_insert] := "Tuples1"!"insert"
     with ffunction "Tuples1_find" reserving 34 [Tuples1_find] := "Tuples1"!"find"
     with ffunction "Tuples1_enumerate" reserving 34 [Tuples1_enumerate] := "Tuples1"!"enumerate"
+
+    with ffunction "Tuples2_new" reserving 7 [Tuples2_new] := "Tuples2"!"new"
+    with ffunction "Tuples2_insert" reserving 31 [Tuples2_insert] := "Tuples2"!"insert"
+    with ffunction "Tuples2_findBoth" reserving 38 [Tuples2_findBoth] := "Tuples2"!"findBoth"
+    with ffunction "Tuples2_findFirst" reserving 37 [Tuples2_findFirst] := "Tuples2"!"findFirst"
+    with ffunction "Tuples2_findSecond" reserving 36 [Tuples2_findSecond] := "Tuples2"!"findSecond"
+    with ffunction "Tuples2_enumerate" reserving 36 [Tuples2_enumerate] := "Tuples2"!"enumerate"
   }}.
 
 Ltac peel := repeat (apply andL || (apply injL; intro) || (apply existsL; intro)); reduce.
@@ -276,6 +290,33 @@ Proof.
   apply Properties.F.empty_mapsto_iff in H6; tauto.
 Qed.
 
+Lemma readd_Tuples2 : forall c len key1 key2 rv rv',
+  tuples2 len key1 key2 rv' c * is_heap heap_empty
+  ===> is_heap (WordMap.add c (Tuples2 len key1 key2 rv') (heap_upd heap_empty c (Tuples2 len key1 key2 rv))).
+Proof.
+  intros.
+  unfold is_heap at 2.
+  assert (List.In (c, Tuples2 len key1 key2 rv') (heap_elements (WordMap.add c (Tuples2 len key1 key2 rv') (heap_upd heap_empty c (Tuples2 len key1 key2 rv))))).
+  apply InA_In.
+  apply WordMap.elements_1.
+  apply WordMap.add_1.
+  auto.
+  eapply starL_in in H; try (apply NoDupA_NoDup; apply WordMap.elements_3w).
+  destruct H; intuition idtac.
+  eapply Himp_trans; [ | apply H0 ].
+  simpl.
+  apply Himp_star_frame; try apply Himp_refl.
+  apply starL_permute; auto.
+  apply NoDupA_NoDup; apply WordMap.elements_3w.
+  intuition.
+  apply H2 in H1; intuition.
+  apply In_InA' in H4.
+  apply WordMap.elements_2 in H4.
+  apply Properties.F.add_mapsto_iff in H4; intuition.
+  apply Properties.F.add_mapsto_iff in H5; intuition.
+  apply Properties.F.empty_mapsto_iff in H6; tauto.
+Qed.
+
 Lemma get_rval'' : forall specs st P (Q : Prop) R S T Z,
   (Q -> interp specs (![P * R * S * T ] st ---> Z)%PropX)
   -> interp specs (![P * (([|Q|] * R) * S) * T] st ---> Z)%PropX.
@@ -416,6 +457,44 @@ Proof.
   unfold is_heap at 2.
   match goal with
   | [ |- context[Bags.starL _ ?x] ] => assert (List.In (c, Tuples1 len key rv') x)
+  end.
+  apply InA_In.
+  apply WordMap.elements_1.
+  apply WordMap.remove_2; auto.
+  apply WordMap.add_1.
+  auto.
+  eapply starL_in in H0; try (apply NoDupA_NoDup; apply WordMap.elements_3w).
+  destruct H0; intuition idtac.
+  eapply Himp_trans; [ | apply H1 ].
+  simpl.
+  apply Himp_star_frame; try apply Himp_refl.
+  apply starL_permute; auto.
+  apply NoDupA_NoDup; apply WordMap.elements_3w.
+  intuition.
+  apply H3 in H2; intuition.
+  apply In_InA' in H5.
+  apply WordMap.elements_2 in H5.
+  apply Properties.F.remove_mapsto_iff in H5; intuition.
+  apply Properties.F.add_mapsto_iff in H6; intuition.
+  apply Properties.F.add_mapsto_iff in H7; intuition.
+  apply Properties.F.add_mapsto_iff in H8; intuition.
+  apply Properties.F.empty_mapsto_iff in H9; tauto.
+Qed.
+
+Lemma readd_Tuples2' : forall c rv rv' c' ov len key1 key2,
+  c <> c'
+  -> tuples2 len key1 key2 rv' c * is_heap heap_empty
+  ===> is_heap
+      (WordMap.remove c'
+         (WordMap.add c (Tuples2 len key1 key2 rv')
+            (WordMap.add c' ov
+               (WordMap.add c (Tuples2 len key1 key2 rv)
+                  heap_empty)))).
+Proof.
+  intros.
+  unfold is_heap at 2.
+  match goal with
+  | [ |- context[Bags.starL _ ?x] ] => assert (List.In (c, Tuples2 len key1 key2 rv') x)
   end.
   apply InA_In.
   apply WordMap.elements_1.
@@ -910,6 +989,131 @@ Proof.
   do_delegate2 ("self" :: nil).
 
 
+  (* Tuples1 *)
+
+  (* new *)
+
+  do_abort ("len" :: "key1" :: "key2" :: nil).
+  do_abort ("len" :: "key1" :: "key2" :: nil).
+  do_abort ("len" :: "key1" :: "key2" :: nil).
+
+  do_delegate1 ("len" :: "key1" :: "key2" :: nil) hints.
+  descend; step auto_ext.
+  peel.
+  descend; step auto_ext.
+  2: returnAdt.
+  simpl.
+  make_toArray ("len" :: "key1" :: "key2" :: nil).
+  step auto_ext.
+  etransitivity; [ | apply (@is_state_in x2) ].
+  unfolder.
+  do_delegate2 ("len" :: "key1" :: "key2" :: nil).
+
+  (* insert *)
+
+  do_abort ("self" :: "tup" :: nil).
+  do_abort ("self" :: "tup" :: nil).
+  do_abort ("self" :: "tup" :: nil).
+
+  do_delegate1 ("self" :: "tup" :: nil) hints.
+  add_side_conditions.
+  descend; step hints.
+  simpl; step hints.
+  peel.
+  apply get_rval''; intro.
+  descend; step hints.
+  descend; step hints.
+  2: returnScalar; eauto 9.
+  simpl.
+  make_toArray ("self" :: "tup" :: nil).
+  step auto_ext.
+  etransitivity; [ | apply (@is_state_in x2) ].
+  unfolder.
+  etransitivity; [ | apply himp_star_frame; [ reflexivity | apply readd_Tuples2' ] ].
+  do_delegate2 ("self" :: "tup" :: nil).
+  congruence.
+
+  (* findBoth *)
+
+  do_abort ("self" :: "k1" :: "k2" :: nil).
+  do_abort ("self" :: "k1" :: "k2" :: nil).
+  do_abort ("self" :: "k1" :: "k2" :: nil).
+
+  do_delegate1 ("self" :: "k1" :: "k2" :: nil) hints.
+  peel.
+  apply get_rval''''; intro.
+  descend; step auto_ext.
+  descend; step auto_ext.
+  2: returnAdt; eauto 10.
+  simpl.
+  make_toArray ("self" :: "k1" :: "k2" :: nil).
+  step auto_ext.
+  etransitivity; [ | apply (@is_state_in x2) ].
+  unfolder.
+  etransitivity; [ | apply himp_star_frame; [ reflexivity | apply readd_Tuples2 ] ].
+  do_delegate2 ("self" :: "k1" :: "k2" :: nil).
+
+  (* findFirst *)
+
+  do_abort ("self" :: "k1" ::  nil).
+  do_abort ("self" :: "k1" ::  nil).
+  do_abort ("self" :: "k1" ::  nil).
+
+  do_delegate1 ("self" :: "k1" ::  nil) hints.
+  peel.
+  apply get_rval''''; intro.
+  descend; step auto_ext.
+  descend; step auto_ext.
+  2: returnAdt; eauto 10.
+  simpl.
+  make_toArray ("self" :: "k1" ::  nil).
+  step auto_ext.
+  etransitivity; [ | apply (@is_state_in x2) ].
+  unfolder.
+  etransitivity; [ | apply himp_star_frame; [ reflexivity | apply readd_Tuples2 ] ].
+  do_delegate2 ("self" :: "k1" ::  nil).
+
+  (* findSecond *)
+
+  do_abort ("self" :: "k2" ::  nil).
+  do_abort ("self" :: "k2" ::  nil).
+  do_abort ("self" :: "k2" ::  nil).
+
+  do_delegate1 ("self" :: "k2" ::  nil) hints.
+  peel.
+  apply get_rval''''; intro.
+  descend; step auto_ext.
+  descend; step auto_ext.
+  2: returnAdt; eauto 10.
+  simpl.
+  make_toArray ("self" :: "k2" ::  nil).
+  step auto_ext.
+  etransitivity; [ | apply (@is_state_in x2) ].
+  unfolder.
+  etransitivity; [ | apply himp_star_frame; [ reflexivity | apply readd_Tuples2 ] ].
+  do_delegate2 ("self" :: "k2" ::  nil).
+
+  (* enumerate *)
+
+  do_abort ("self" :: nil).
+  do_abort ("self" :: nil).
+  do_abort ("self" :: nil).
+
+  do_delegate1 ("self" :: nil) hints.
+  peel.
+  apply get_rval''''; intro.
+  descend; step auto_ext.
+  descend; step auto_ext.
+  2: returnAdt; eauto 8.
+  simpl.
+  make_toArray ("self" :: nil).
+  step auto_ext.
+  etransitivity; [ | apply (@is_state_in x2) ].
+  unfolder.
+  etransitivity; [ | apply himp_star_frame; [ reflexivity | apply readd_Tuples2 ] ].
+  do_delegate2 ("self" :: nil).
+
+
   (* Grabby time *)
   Grab Existential Variables.
   exact 0.
@@ -925,7 +1129,8 @@ Definition m1 := link ArrayTupleF.m m0.
 Definition m2 := link TupleListF.m m1.
 Definition m3 := link Tuples0F.m m2.
 Definition m4 := link Tuples1F.m m3.
-Definition m := link Malloc.m m4.
+Definition m5 := link Tuples2F.m m4.
+Definition m := link Malloc.m m5.
 
 Theorem ok1 : moduleOk m1.
 Proof.
@@ -947,7 +1152,12 @@ Proof.
   link Tuples1F.ok ok3.
 Qed.
 
+Theorem ok5 : moduleOk m5.
+Proof.
+  link Tuples2F.ok ok4.
+Qed.
+
 Theorem ok : moduleOk m.
 Proof.
-  link Malloc.ok ok4.
+  link Malloc.ok ok5.
 Qed.
